Some changes in LRs

theories/L6_PCPS/bounds.v
@@ -1,8 +1,7 @@
 Require Import Coq.NArith.BinNat Coq.Relations.Relations Coq.MSets.MSets Coq.MSets.MSetRBT
         Coq.Lists.List Coq.omega.Omega Coq.Sets.Ensembles.
 
-Require Import L6.cps L6.eval L6.cps_util L6.identifiers L6.ctx
-        L6.Ensembles_util L6.List_util L6.size_cps L6.tactics L6.set_util
+Require Import L6.cps L6.eval L6.Ensembles_util L6.List_util L6.tactics L6.set_util
         L6.logical_relations L6.logical_relations_cc.
 
 Import ListNotations.
@@ -10,36 +9,110 @@ Import ListNotations.
 
 Section Bounds. 
 
-  Context (K : nat) (* in essence, the number of inlined applications *)
-          (M : nat) (* The total overhead of all L6 transformations, generally different for each program *)
-          (Kpos : K > 0) (Mpos : M > 0).
+  Context (K : nat -> env -> exp -> nat) (* in essence, the number of inlined applications *)
+          (M : nat -> env -> exp -> nat). (* The total overhead of all L6 transformations, generally different for each program *)
+          
   (* TODO: maybe remove step-index k if not needed in bounds *)
 
-  Definition upper_boundG : relation (exp * env *  nat) := 
-    fun '(e1, rho1, c1) '(e2, rho2, c2) => c2 <= M * c1.
+  Definition upper_boundG (k : nat) : relation (exp * env *  nat) := 
+    fun '(e1, rho1, c1) '(e2, rho2, c2) => c2 <= (M k rho1 e1) * (c1 + 1).
 
-  Definition lower_boundG : relation (exp * env * nat) := 
-    fun '(e1, rho1, c1) '(e2, rho2, c2) => c1 <= K * c2.
+  Definition lower_boundG (k : nat) : relation (exp * env * nat) := 
+    fun '(e1, rho1, c1) '(e2, rho2, c2) => c1 <= (K k rho1 e1) * (c2 + 1).
 
-  Definition boundG : relation (exp * env *  nat) :=
-    relation_conjunction lower_boundG upper_boundG.
+  (* + 1 is needed in the lower bound ecause sourvce might time out 
+   * in say M steps but that may be 0 steps in target *)
+
+  (* + 1 is not technically needed in the upper bound but it makes 
+    things easier *)
+
+  Definition boundG (k : nat) : relation (exp * env *  nat) :=
+    relation_conjunction (lower_boundG k) (upper_boundG k).
  
-  Definition upper_boundL (local : nat) : relation nat := 
-    fun c1 c2 => c2 + local <= M * c1.
+  Definition upper_boundL (local : nat) (k : nat) (rho : env) (e : exp) : relation nat := 
+    fun c1 c2 => c2 + local <= M k rho e * (c1 + 1).
 
-  Definition lower_boundL (local : nat) : relation nat := 
-    fun c1 c2 => c1 <= K * (c2 + local).
+  Definition lower_boundL (local : nat) (k : nat) (rho : env) (e : exp) : relation nat := 
+    fun c1 c2 => c1 <= K k rho e * (c2 + 1 + local).
 
-  Definition boundL (local : nat) : relation nat :=
-    relation_conjunction (lower_boundL local) (upper_boundL local).
+  Definition boundL (local : nat) (k : nat) (rho : env) (e : exp) : relation nat :=
+    relation_conjunction (lower_boundL local k rho e) (upper_boundL local k rho e).
   
+  (* bound properties *)
+  
+  Lemma boundL_0_implies_boundG k e1 e2 rho1 rho2 c1 c2 : 
+    boundL 0 k rho1 e1 c1 c2 -> boundG k (e1, rho1, c1) (e2, rho2, c2).
+  Proof.
+    unfold boundL, boundG, lower_boundL, lower_boundG, upper_boundL, upper_boundG. 
+    intros [H1 H2]. split; eauto.
+    eapply le_trans. eassumption. 
+    eapply Nat_as_OT.mul_le_mono_l. omega. 
+    rewrite Nat_as_DT.add_0_r in H2. 
+    eapply le_trans. eassumption. 
+    eapply Nat_as_OT.mul_le_mono_l. omega.       
+  Qed.
+
+  Lemma post_compat_relation_conj P1 P2 Q1 Q2 :
+    post_compat P1 Q1 ->
+    post_compat P2 Q2 ->
+    post_compat (relation_conjunction P1 P2) (relation_conjunction Q1 Q2).
+  Proof.
+    intros H1 H2 x y z [Hr1 Hr2]. split; eauto.
+  Qed.
+
+  Lemma post_refl_relation_conj P1 P2 :
+    post_refl P1 ->
+    post_refl P2 ->
+    post_refl (relation_conjunction P1 P2).
+  Proof.
+    intros H1 H2 x. split; eauto.
+  Qed. 
+
+  Context (Kpos : K > 0) (Mpos : M > 0).
+
+  Lemma boundL_post_compat l :
+    post_compat (boundL l) (boundL l). 
+  Proof.
+    unfold boundL. eapply post_compat_relation_conj.
+    - intros x y z Hl.  
+      unfold boundL, boundG, lower_boundL, lower_boundG, upper_boundL, upper_boundG  in *. 
+      eapply le_trans. eapply plus_le_compat_r. eassumption.
+      replace (y + z + 1 + l) with (y + 1 + l + z) by omega.
+      rewrite Nat_as_OT.mul_add_distr_l with (p := z).
+      eapply plus_le_compat_l. 
+      assert (Hyp := mult_O_le z K). inv Hyp; eauto. omega.
+    - intros x y z Hl.  
+      unfold boundL, boundG, lower_boundL, lower_boundG, upper_boundL, upper_boundG  in *. 
+      replace (y + z + l) with (y + l + z) by omega.
+      eapply le_trans. eapply plus_le_compat_r. eassumption.
+      replace (x + z + 1) with (x + 1 + z) by omega.
+      rewrite Nat_as_OT.mul_add_distr_l with (p := z).
+      eapply plus_le_compat_l. 
+      assert (Hyp := mult_O_le z M). inv Hyp; eauto. omega.
+  Qed. 
+  
+  Lemma boundL_post_refl l :
+    l <= M ->
+    post_refl (boundL l). 
+  Proof.
+    intros Hle. unfold boundL. 
+    eapply post_refl_relation_conj; unfold boundL, boundG, lower_boundL, lower_boundG, upper_boundL, upper_boundG  in *. 
+    - intros x. rewrite !Nat_as_OT.mul_add_distr_l.
+      assert (Hyp := mult_O_le x K). inv Hyp; eauto. omega.
+      eapply le_trans. eassumption. 
+      rewrite <- plus_assoc. eapply le_plus_l.
+    - intros x. rewrite !Nat_as_OT.mul_add_distr_l.
+      assert (Hyp := mult_O_le x M). inv Hyp; eauto. omega.
+      eapply plus_le_compat. eassumption. omega.
+  Qed.
+
   (* Divergence preservation *)
   Lemma cc_approx_exp_divergence pr cenv ct l e1 rho1 e2 rho2 :  
     (forall k, cc_approx_exp pr cenv ct k (boundL l) boundG (e1, rho1) (e2, rho2)) ->
     diverge pr cenv rho1 e1 -> 
     diverge pr cenv rho2 e2.
   Proof.
-    intros Hexp H1 c2. assert (Hd := H1). specialize (H1 (K*(c2 + l))).
+    intros Hexp H1 c2. assert (Hd := H1). specialize (H1 (K*(c2 + 1 + l))).
     edestruct Hexp as [v2 [c2' [Hs2 [Hp Hval]]]]. reflexivity. eassumption.
     destruct v2; try contradiction.
     assert (Hleq : c2 <= c2').
@@ -47,7 +120,8 @@ Section Bounds.
       eapply Nat_as_DT.mul_le_mono_pos_l in Hp1; eauto. omega. }
     eapply bstep_fuel_OOT_monotonic; eassumption. 
   Qed.
-  
+
+
 End Bounds.
 
   
